lib/DataStructures/MutableBtreeBulkOperations.i.dfy
@@ -12,9 +12,9 @@ abstract module MutableBtreeBulkOperations {
   
   method NumElements(node: Node) returns (count: uint64)
     requires WFShape(node)
-    requires Spec.WF(I(node))
-    requires Spec.NumElements(I(node)) < Uint64UpperBound()
-    ensures count as nat == Spec.NumElements(I(node))
+    requires Model.WF(I(node))
+    requires Model.NumElements(I(node)) < Uint64UpperBound()
+    ensures count as nat == Model.NumElements(I(node))
     decreases node.height
   {
     reveal_I();
@@ -28,14 +28,14 @@ abstract module MutableBtreeBulkOperations {
       var i: uint64 := 0;
       while i < node.contents.nchildren
         invariant i <= node.contents.nchildren
-        invariant icount == Spec.NumElementsOfChildren(inode.children[..i])
+        invariant icount == Model.NumElementsOfChildren(inode.children[..i])
         invariant icount < Uint64UpperBound()
         invariant count == icount as uint64
       {
-        ghost var ichildcount := Spec.NumElements(inode.children[i]);
+        ghost var ichildcount := Model.NumElements(inode.children[i]);
         assert inode.children[..i+1][..i] == inode.children[..i];
-        Spec.NumElementsOfChildrenNotZero(inode);
-        Spec.NumElementsOfChildrenDecreases(inode.children, (i+1) as int);
+        Model.NumElementsOfChildrenNotZero(inode);
+        Model.NumElementsOfChildrenDecreases(inode.children, (i+1) as int);
         icount := icount + ichildcount;
 
         IOfChild(node, i as int);
@@ -53,14 +53,14 @@ abstract module MutableBtreeBulkOperations {
     requires keys.Length == values.Length
     requires keys !in node.repr
     requires values !in node.repr
-    requires start as nat + Spec.NumElements(I(node)) <= keys.Length
-    requires start as nat + Spec.NumElements(I(node)) < Uint64UpperBound()
-    ensures nextstart as nat == start as nat + Spec.NumElements(I(node))
+    requires start as nat + Model.NumElements(I(node)) <= keys.Length
+    requires start as nat + Model.NumElements(I(node)) < Uint64UpperBound()
+    ensures nextstart as nat == start as nat + Model.NumElements(I(node))
     ensures keys[..start] == old(keys[..start])
-    ensures keys[start..nextstart] == Spec.ToSeq(I(node)).0
+    ensures keys[start..nextstart] == Model.ToSeq(I(node)).0
     ensures keys[nextstart..] == old(keys[nextstart..]);
     ensures values[..start] == old(values[..start]);
-    ensures values[start..nextstart] == Spec.ToSeq(I(node)).1
+    ensures values[start..nextstart] == Model.ToSeq(I(node)).1
     ensures values[nextstart..] == old(values[nextstart..])
     modifies keys, values
     decreases node.height
@@ -70,46 +70,46 @@ abstract module MutableBtreeBulkOperations {
       Arrays.Memcpy(values, start, node.contents.values[..node.contents.nkeys]); // FIXME: remove conversion to seq
       nextstart := start + node.contents.nkeys;
       forall
-        ensures keys[start..nextstart] == Spec.ToSeq(I(node)).0
-        ensures values[start..nextstart] == Spec.ToSeq(I(node)).1
+        ensures keys[start..nextstart] == Model.ToSeq(I(node)).0
+        ensures values[start..nextstart] == Model.ToSeq(I(node)).1
       {
         reveal_I();
-        Spec.reveal_ToSeq();
+        Model.reveal_ToSeq();
       }
     } else {
       nextstart := start;
       var i: uint64 := 0;
       while i < node.contents.nchildren
         invariant 0 <= i <= node.contents.nchildren
-        invariant nextstart as nat == start as nat + Spec.NumElementsOfChildren(I(node).children[..i])
+        invariant nextstart as nat == start as nat + Model.NumElementsOfChildren(I(node).children[..i])
         invariant nextstart as nat <= keys.Length
         invariant keys[..start] == old(keys[..start])
-        invariant keys[start..nextstart] == Spec.Seq.Flatten(Spec.ToSeqChildren(I(node).children[..i]).0)
+        invariant keys[start..nextstart] == Model.Seq.Flatten(Model.ToSeqChildren(I(node).children[..i]).0)
         invariant keys[nextstart..] == old(keys[nextstart..]);
         invariant values[..start] == old(values[..start]);
-        invariant values[start..nextstart] == Spec.Seq.Flatten(Spec.ToSeqChildren(I(node).children[..i]).1)
+        invariant values[start..nextstart] == Model.Seq.Flatten(Model.ToSeqChildren(I(node).children[..i]).1)
         invariant values[nextstart..] == old(values[nextstart..])
       {
         assert WFShapeChildren(node.contents.children[..node.contents.nchildren], node.repr, node.height);
         assert I(node).children[..i+1][..i] == I(node).children[..i];
-        Spec.NumElementsOfChildrenDecreases(I(node).children, (i + 1) as int);
-        Spec.ToSeqChildrenDecomposition(I(node).children[..i+1]);
+        Model.NumElementsOfChildrenDecreases(I(node).children, (i + 1) as int);
+        Model.ToSeqChildrenDecomposition(I(node).children[..i+1]);
         IOfChild(node, i as int);
 
         nextstart := ToSeqSubtree(node.contents.children[i], keys, values, nextstart);
         i := i + 1;
-        Spec.reveal_ToSeq();
+        Model.reveal_ToSeq();
       }
       assert I(node).children[..node.contents.nchildren] == I(node).children;
-      Spec.reveal_ToSeq();
+      Model.reveal_ToSeq();
     }
   }
 
   method ToSeq(node: Node) returns (kvlists: (array<Key>, array<Value>))
     requires WFShape(node)
-    requires Spec.WF(I(node))
-    requires Spec.NumElements(I(node)) < Uint64UpperBound()
-    ensures (kvlists.0[..], kvlists.1[..]) == Spec.ToSeq(I(node))
+    requires Model.WF(I(node))
+    requires Model.NumElements(I(node)) < Uint64UpperBound()
+    ensures (kvlists.0[..], kvlists.1[..]) == Model.ToSeq(I(node))
     ensures fresh(kvlists.0)
     ensures fresh(kvlists.1)
   {
@@ -140,7 +140,7 @@ abstract module MutableBtreeBulkOperations {
 
   predicate ValidBoundariesForSeqInner(len: uint64, boundaries: seq<uint64>)
   {
-    Spec.ValidBoundariesForSeq(len as nat, NatBoundaries(boundaries))
+    Model.ValidBoundariesForSeq(len as nat, NatBoundaries(boundaries))
   }
   
   lemma ValidBoundariesForSeqProperties(len: uint64, boundaries: seq<uint64>)
@@ -165,7 +165,7 @@ abstract module MutableBtreeBulkOperations {
   
   predicate BoundariesFit(boundaries: seq<uint64>, groupSize: uint64)
   {
-    Spec.BoundariesFit(NatBoundaries(boundaries), groupSize as nat)
+    Model.BoundariesFit(NatBoundaries(boundaries), groupSize as nat)
   }
   
   // FIXME: This proof is bizarre and fragile.
@@ -173,7 +173,7 @@ abstract module MutableBtreeBulkOperations {
     requires 0 < numthings
     requires 0 < groupSize
     requires numthings as int + groupSize as int < Uint64UpperBound()
-    ensures NatBoundaries(boundaries) == Spec.BuildBoundaries(numthings as nat, groupSize as nat)
+    ensures NatBoundaries(boundaries) == Model.BuildBoundaries(numthings as nat, groupSize as nat)
   {
     var numgroups: uint64 := (numthings + groupSize - 1) / groupSize;
     var aboundaries := newArrayFill(numgroups + 1, numthings);
@@ -181,13 +181,13 @@ abstract module MutableBtreeBulkOperations {
     ghost var nnumthings := numthings as nat;
     ghost var ngroupSize := groupSize as nat;
     ghost var targetA: seq<nat> := Apply((i: nat) => i * ngroupSize, Range((nnumthings + ngroupSize - 1) / ngroupSize));
-    ghost var target := Spec.BuildBoundaries(nnumthings, ngroupSize);
+    ghost var target := Model.BuildBoundaries(nnumthings, ngroupSize);
 
-    assert target == targetA || target == targetA + [nnumthings] by {Spec.reveal_BuildBoundariesInner();}
+    assert target == targetA || target == targetA + [nnumthings] by {Model.reveal_BuildBoundariesInner();}
     assert target ==
       if Last(targetA) == nnumthings then targetA
       else targetA + [nnumthings]
-    by { Spec.reveal_BuildBoundariesInner(); }
+    by { Model.reveal_BuildBoundariesInner(); }
 
     var i: uint64 := 0;
     while i < numgroups
@@ -211,10 +211,10 @@ abstract module MutableBtreeBulkOperations {
     requires |pivots| + 1 < Uint64UpperBound()
     requires ValidBoundariesForSeq(|pivots| as uint64 + 1, boundaries)
     requires |boundaries| < Uint64UpperBound()
-    ensures subpivots == Spec.ExtractPivotsForBoundaries(pivots, NatBoundaries(boundaries))
+    ensures subpivots == Model.ExtractPivotsForBoundaries(pivots, NatBoundaries(boundaries))
   {
-    ghost var target := Spec.ExtractPivotsForBoundaries(pivots, NatBoundaries(boundaries));
-    Spec.reveal_ExtractPivotsForBoundaries();
+    ghost var target := Model.ExtractPivotsForBoundaries(pivots, NatBoundaries(boundaries));
+    Model.reveal_ExtractPivotsForBoundaries();
 
     var asubpivots := newArrayFill(|boundaries| as uint64 - 2, DefaultKey());
 
@@ -230,40 +230,40 @@ abstract module MutableBtreeBulkOperations {
     subpivots := asubpivots[..];
   }
 
-  method BuildLeafForSequence(kvlist: Spec.KVList, boundaries: seq<uint64>, i: uint64) returns (node: Node)
+  method BuildLeafForSequence(kvlist: Model.KVList, boundaries: seq<uint64>, i: uint64) returns (node: Node)
     requires |kvlist.keys| < Uint64UpperBound()
-    requires Spec.WFKVList(kvlist)
+    requires Model.WFKVList(kvlist)
     requires ValidBoundariesForSeq(|kvlist.keys| as uint64, boundaries)
     requires i as int < |boundaries| - 1
     requires BoundariesFit(boundaries, MaxKeysPerLeaf())
     ensures WFShape(node)
-    ensures I(node) == Spec.BuildLeafForSequence(kvlist, NatBoundaries(boundaries), i as nat)
+    ensures I(node) == Model.BuildLeafForSequence(kvlist, NatBoundaries(boundaries), i as nat)
     ensures fresh(node.repr)
   {
-    Spec.ValidBoundaryLength(|kvlist.keys|, NatBoundaries(boundaries));
+    Model.ValidBoundaryLength(|kvlist.keys|, NatBoundaries(boundaries));
     Uint64_Order.IsStrictlySortedImpliesLte(boundaries, i as int, i as int + 1);
-    assert boundaries[i+1] - boundaries[i] <= MaxKeysPerLeaf() by { Spec.reveal_BoundariesFit(); }
+    assert boundaries[i+1] - boundaries[i] <= MaxKeysPerLeaf() by { Model.reveal_BoundariesFit(); }
     
     var mykeys := kvlist.keys[boundaries[i]..boundaries[i+1]];
     var myvals := kvlist.values[boundaries[i]..boundaries[i+1]];
     node := LeafFromSeqs(mykeys, myvals);
 
-    Spec.reveal_ExtractBoundedSubsequence();
+    Model.reveal_ExtractBoundedSubsequence();
   }
 
-  method BuildLeavesForSequence(kvlist: Spec.KVList, boundaries: seq<uint64>) returns (nodes: seq<Node>)
-    requires Spec.WFKVList(kvlist)
+  method BuildLeavesForSequence(kvlist: Model.KVList, boundaries: seq<uint64>) returns (nodes: seq<Node>)
+    requires Model.WFKVList(kvlist)
     requires |kvlist.keys| < Uint64UpperBound() - 1
     requires ValidBoundariesForSeq(|kvlist.keys| as uint64, boundaries)
     requires BoundariesFit(boundaries, MaxKeysPerLeaf())
     ensures WFShapeSiblings(nodes)
     ensures fresh(SeqRepr(nodes))
     ensures forall i :: 0 <= i < |nodes| ==> nodes[i].height  == 0
-    ensures ISiblings(nodes) == Spec.BuildLeavesForSequence(kvlist, NatBoundaries(boundaries))
+    ensures ISiblings(nodes) == Model.BuildLeavesForSequence(kvlist, NatBoundaries(boundaries))
   {
-    Spec.ValidBoundaryLength(|kvlist.keys|, NatBoundaries(boundaries));
+    Model.ValidBoundaryLength(|kvlist.keys|, NatBoundaries(boundaries));
     var anodes: array<Node?> := newArrayFill(|boundaries| as uint64 - 1, null);
-    ghost var target := Spec.BuildLeavesForSequence(kvlist, NatBoundaries(boundaries));
+    ghost var target := Model.BuildLeavesForSequence(kvlist, NatBoundaries(boundaries));
     
     var i: uint64 := 0;
     while i < anodes.Length as uint64
@@ -273,7 +273,7 @@ abstract module MutableBtreeBulkOperations {
       invariant WFShapeSiblings(anodes[..i])
       invariant fresh(SeqRepr(anodes[..i]))
       invariant forall j :: 0 <= j < i ==> anodes[j].height == 0
-      invariant ISiblings(anodes[..i]) == Spec.BuildLeavesForSequenceInner(kvlist, NatBoundaries(boundaries), i as int);
+      invariant ISiblings(anodes[..i]) == Model.BuildLeavesForSequenceInner(kvlist, NatBoundaries(boundaries), i as int);
     {
       anodes[i] := BuildLeafForSequence(kvlist, boundaries, i);
       i := i + 1;
@@ -309,7 +309,7 @@ abstract module MutableBtreeBulkOperations {
     requires ValidBoundariesForSeq(|things| as uint64, boundaries)
     requires 0 <= i as int < |boundaries|-1
   {
-    Spec.ExtractBoundedSubsequence(things, NatBoundaries(boundaries), i as int)
+    Model.ExtractBoundedSubsequence(things, NatBoundaries(boundaries), i as int)
   }
 
   lemma ExtractBoundedSubsequenceFacts<T>(things: seq<T>, boundaries: seq<uint64>, i: uint64)
@@ -320,9 +320,9 @@ abstract module MutableBtreeBulkOperations {
     ensures boundaries[i] < boundaries[i+1]
     ensures ExtractBoundedSubsequence(things, boundaries, i) == things[boundaries[i]..boundaries[i+1]]
   {
-    Spec.ValidBoundaryLength(|things|, NatBoundaries(boundaries));
+    Model.ValidBoundaryLength(|things|, NatBoundaries(boundaries));
     Uint64_Order.IsStrictlySortedImpliesLt(boundaries, i as int, i as int + 1);
-    Spec.reveal_ExtractBoundedSubsequence();
+    Model.reveal_ExtractBoundedSubsequence();
   }
     
   lemma ExtractBoundedSubsequenceRepr(nodes: seq<Node>, boundaries: seq<uint64>, i: uint64)
@@ -349,9 +349,9 @@ abstract module MutableBtreeBulkOperations {
     && |bpa.children| < Uint64UpperBound() - 1
     && WFShapeSiblings(bpa.children)
     && (forall j :: 0 <= j < |bpa.children| ==> bpa.children[j].height < bpa.height)
-    && Spec.WF(Spec.Index(bpa.pivots, ISiblings(bpa.children)))
+    && Model.WF(Model.Index(bpa.pivots, ISiblings(bpa.children)))
     && ValidBoundariesForSeq(|bpa.children| as uint64, bpa.boundaries)
-    && (Spec.ValidBoundaryLength(|bpa.children|, NatBoundaries(bpa.boundaries));
+    && (Model.ValidBoundaryLength(|bpa.children|, NatBoundaries(bpa.boundaries));
        && BoundariesFit(bpa.boundaries, MaxChildren()))
   }
 
@@ -373,23 +373,23 @@ abstract module MutableBtreeBulkOperations {
     && fresh(parent.repr - SeqRepr(mychildren))
   }
 
-  predicate MatchesSpecBuildParent(bpa: BuildParentsArgs, i: uint64, parent: Node)
+  predicate MatchesModelBuildParent(bpa: BuildParentsArgs, i: uint64, parent: Node)
     requires BuildParentRequires(bpa, i)
     requires WFShape(parent)
     reads Set(bpa.children), SeqRepr(bpa.children), parent, parent.repr
   {
-    I(parent) == Spec.BuildParent(ISiblings(bpa.children), bpa.pivots, NatBoundaries(bpa.boundaries), i as nat)
+    I(parent) == Model.BuildParent(ISiblings(bpa.children), bpa.pivots, NatBoundaries(bpa.boundaries), i as nat)
   }
   
   method BuildParent(bpa: BuildParentsArgs, i: uint64) returns (parent: Node)
     requires BuildParentRequires(bpa, i)
     ensures BuildParentShapeProperties(bpa, i, parent)
-    ensures MatchesSpecBuildParent(bpa, i, parent)
+    ensures MatchesModelBuildParent(bpa, i, parent)
   {
     ExtractBoundedSubsequenceFacts(bpa.children, bpa.boundaries, i);
     var mychildren := bpa.children[bpa.boundaries[i]..bpa.boundaries[i+1]];
     var mypivots   := bpa.pivots[bpa.boundaries[i]..bpa.boundaries[i+1]-1];
-    assert |mychildren| <= MaxChildren() as int by { Spec.reveal_BoundariesFit(); }
+    assert |mychildren| <= MaxChildren() as int by { Model.reveal_BoundariesFit(); }
     parent := IndexFromChildren(mypivots, mychildren, bpa.height);
     forall j, k | 0 <= j < k < |mychildren|
       ensures DisjointReprs(mychildren, j, k)
@@ -402,7 +402,7 @@ abstract module MutableBtreeBulkOperations {
     assert WFShape(parent);
     reveal_I();
     ghost var iparent := I(parent);
-    ghost var target := Spec.BuildParent(ISiblings(bpa.children), bpa.pivots, NatBoundaries(bpa.boundaries), i as nat);
+    ghost var target := Model.BuildParent(ISiblings(bpa.children), bpa.pivots, NatBoundaries(bpa.boundaries), i as nat);
     assert iparent.pivots == target.pivots;
   }
 
@@ -441,7 +441,7 @@ abstract module MutableBtreeBulkOperations {
   // {
   //   // && (forall j :: 0 <= j < i ==> aparents[j].contents.Index?)
   //   // && (forall j :: 0 <= j < i ==>
-  //   //   var subchildren := Spec.ExtractBoundedSubsequence(children, NatBoundaries(boundaries), j as int);
+  //   //   var subchildren := Model.ExtractBoundedSubsequence(children, NatBoundaries(boundaries), j as int);
   //   //   assume Set(subchildren) <= Set(children);
   //   //   fresh(aparents[j].repr - SeqRepr(subchildren)))
   //   && fresh(allReprs - SeqRepr(children))
@@ -485,12 +485,12 @@ abstract module MutableBtreeBulkOperations {
   //       } else {
   //         assert o in sparents[i].repr - SeqRepr(children);
   //         SubSeqRepr(children, boundaries[i] as nat, boundaries[i+1] as nat);
-  //         assert Spec.ExtractBoundedSubsequence(children, NatBoundaries(boundaries), i as int) ==
+  //         assert Model.ExtractBoundedSubsequence(children, NatBoundaries(boundaries), i as int) ==
   //           children[boundaries[i]..boundaries[i+1]] by {
-  //             Spec.reveal_ExtractBoundedSubsequence();
+  //             Model.reveal_ExtractBoundedSubsequence();
   //         }
   //         assert o in sparents[i].repr -
-  //           SeqRepr(Spec.ExtractBoundedSubsequence(children, NatBoundaries(boundaries), i as int));
+  //           SeqRepr(Model.ExtractBoundedSubsequence(children, NatBoundaries(boundaries), i as int));
   //         assert o == sparents[i] || o == sparents[i].contents.pivots || o == sparents[i].contents.children;
   //       }
   //   }
@@ -615,7 +615,7 @@ abstract module MutableBtreeBulkOperations {
     requires ValidBuildParentsArgs(bpa)
     ensures WFShapeSiblings(parents)
     ensures fresh(SeqRepr(parents) - SeqRepr(bpa.children))
-    ensures ISiblings(parents) == Spec.BuildParents(ISiblings(bpa.children), bpa.pivots, NatBoundaries(bpa.boundaries))
+    ensures ISiblings(parents) == Model.BuildParents(ISiblings(bpa.children), bpa.pivots, NatBoundaries(bpa.boundaries))
     ensures |parents| < |bpa.children|
   {
     // assert Stale(SeqRepr(bpa.children)) by {
@@ -659,9 +659,9 @@ abstract module MutableBtreeBulkOperations {
     requires |children| < Uint64UpperBound() - 1
     requires |children| == |pivots| + 1
     requires WFShapeSiblings(children)
-    requires Spec.WF(Spec.Index(pivots, ISiblings(children)))
+    requires Model.WF(Model.Index(pivots, ISiblings(children)))
     ensures WF(newnode)
-    ensures Interpretation(newnode) == Spec.Interpretation(Spec.Index(pivots, ISiblings(children)))
+    ensures Interpretation(newnode) == Model.Interpretation(Model.Index(pivots, ISiblings(children)))
   {
     var currChildren := children;
     var currPivots := pivots;
@@ -672,7 +672,7 @@ abstract module MutableBtreeBulkOperations {
       //invariant |currChildren| < Uint64UpperBound() - 1
       //invariant |currChildren| == |currPivots| + 1
       //invariant WFShapeSiblings(currChildren)
-      //invariant Spec.WF(Spec.Index(currPivots, ISiblings(currChildren)))
+      //invariant Model.WF(Model.Index(currPivots, ISiblings(currChildren)))
       decreases |currChildren|
     {
       assume false;
@@ -690,11 +690,11 @@ abstract module MutableBtreeBulkOperations {
     assume false;
   }
 
-  method BuildTreeForSequence(kvlist: Spec.KVList) returns (node: Node)
+  method BuildTreeForSequence(kvlist: Model.KVList) returns (node: Node)
     requires 0 < |kvlist.keys| < Uint64UpperBound() - 1
-    requires Spec.WFKVList(kvlist)
+    requires Model.WFKVList(kvlist)
     ensures WF(node)
-    ensures Interpretation(node) == Spec.KVListInterpretation(kvlist)
+    ensures Interpretation(node) == Model.KVListInterpretation(kvlist)
     ensures fresh(node.repr)
   {
     assume false;
@@ -707,21 +707,21 @@ abstract module MutableBtreeBulkOperations {
     
   // method SplitLeafOfIndexAtKey(node: Node, childidx: uint64, pivot: Key, nleft: uint64)  returns (ghost wit: Key)
   //   requires WFShape(node)
-  //   requires Spec.WF(I(node))
+  //   requires Model.WF(I(node))
   //   requires node.contents.Index?
   //   requires !Full(node)
   //   requires 0 <= childidx < node.contents.nchildren
   //   requires node.contents.children[childidx].contents.Leaf?
   //   requires WFShape(node.contents.children[childidx])
-  //   requires Spec.Keys.lt(node.contents.children[childidx].contents.keys[0], pivot)
-  //   requires Spec.Keys.lte(pivot, node.contents.children[childidx].contents.keys[node.contents.children[childidx].contents.nkeys-1])
-  //   requires Spec.Keys.IsSorted(node.contents.children[childidx].contents.keys[..node.contents.children[childidx].contents.nkeys])
-  //   requires nleft as int == Spec.Keys.LargestLt(node.contents.children[childidx].contents.keys[..node.contents.children[childidx].contents.nkeys], pivot) + 1
+  //   requires Model.Keys.lt(node.contents.children[childidx].contents.keys[0], pivot)
+  //   requires Model.Keys.lte(pivot, node.contents.children[childidx].contents.keys[node.contents.children[childidx].contents.nkeys-1])
+  //   requires Model.Keys.IsSorted(node.contents.children[childidx].contents.keys[..node.contents.children[childidx].contents.nkeys])
+  //   requires nleft as int == Model.Keys.LargestLt(node.contents.children[childidx].contents.keys[..node.contents.children[childidx].contents.nkeys], pivot) + 1
   //   ensures WFShape(node)
   //   ensures node.contents.Index?
   //   ensures fresh(node.repr - old(node.repr))
   //   ensures node.height == old(node.height)
-  //   ensures Spec.SplitChildOfIndex(old(I(node)), I(node), childidx as int, wit)
+  //   ensures Model.SplitChildOfIndex(old(I(node)), I(node), childidx as int, wit)
   //   ensures !Full(node.contents.children[childidx])
   //   ensures !Full(node.contents.children[childidx+1])
   //   ensures node.contents.pivots[childidx] == pivot
@@ -815,32 +815,32 @@ abstract module MutableBtreeBulkOperations {
 
   // method EnsurePivotNotFullParentOfLeaf(node: Node, pivot: Key, childidx: uint64) returns (pos: int64)
   //   requires WFShape(node)
-  //   requires Spec.WF(I(node))
-  //   requires Spec.NumElements(I(node)) < Uint64UpperBound()
+  //   requires Model.WF(I(node))
+  //   requires Model.NumElements(I(node)) < Uint64UpperBound()
   //   requires node.contents.Index?
   //   requires !Full(node)
-  //   requires childidx as int == Spec.Keys.LargestLte(node.contents.pivots[..node.contents.nchildren-1], pivot) + 1
+  //   requires childidx as int == Model.Keys.LargestLte(node.contents.pivots[..node.contents.nchildren-1], pivot) + 1
   //   requires node.contents.children[childidx].contents.Leaf?
   //   ensures WFShape(node)
-  //   ensures Spec.WF(I(node))
+  //   ensures Model.WF(I(node))
   //   ensures node.contents.Index?
   //   ensures node.height == old(node.height)
   //   ensures fresh(node.repr - old(node.repr))
   //   ensures -1 <= pos as int < node.contents.nchildren as int
   //   ensures 0 <= pos as int < node.contents.nchildren as int - 1 ==> node.contents.pivots[pos] == pivot
-  //   ensures Spec.Interpretation(I(node)) == Spec.Interpretation(old(I(node)))
-  //   ensures Spec.AllKeys(I(node)) <= Spec.AllKeys(old(I(node))) + {pivot}
+  //   ensures Model.Interpretation(I(node)) == Model.Interpretation(old(I(node)))
+  //   ensures Model.AllKeys(I(node)) <= Model.AllKeys(old(I(node))) + {pivot}
   //   modifies node, node.contents.pivots, node.contents.children, node.contents.children[childidx]
   // {
   //   var child := node.contents.children[childidx];
   //   assert child.contents.keys[0..child.contents.nkeys] == child.contents.keys[..child.contents.nkeys];
-  //   var nleft := Spec.Keys.ArrayLargestLtPlus1(child.contents.keys, 0, child.contents.nkeys, pivot);
+  //   var nleft := Model.Keys.ArrayLargestLtPlus1(child.contents.keys, 0, child.contents.nkeys, pivot);
 
   //   if 0 == nleft {
   //     if 0 < childidx {
   //       node.contents.pivots[childidx-1] := pivot;
-  //       assert I(node) == Spec.ReplacePivot(old(I(node)), childidx as int - 1, pivot);
-  //       Spec.IncreasePivotIsCorrect(old(I(node)), childidx as int - 1, pivot);
+  //       assert I(node) == Model.ReplacePivot(old(I(node)), childidx as int - 1, pivot);
+  //       Model.IncreasePivotIsCorrect(old(I(node)), childidx as int - 1, pivot);
   //       pos := childidx as int64 - 1;
   //     } else {
   //       pos := -1;
@@ -848,8 +848,8 @@ abstract module MutableBtreeBulkOperations {
   //   } else if nleft == child.contents.nkeys {
   //     if childidx < node.contents.nchildren-1 {
   //       node.contents.pivots[childidx] := pivot;
-  //       assert I(node) == Spec.ReplacePivot(old(I(node)), childidx as int, pivot);
-  //       Spec.DecreasePivotIsCorrect(old(I(node)), childidx as int, pivot);
+  //       assert I(node) == Model.ReplacePivot(old(I(node)), childidx as int, pivot);
+  //       Model.DecreasePivotIsCorrect(old(I(node)), childidx as int, pivot);
   //       pos := childidx as int64;
   //     } else {
   //       pos := node.contents.nchildren as int64 - 1;
@@ -857,24 +857,24 @@ abstract module MutableBtreeBulkOperations {
   //   } else {
   //     ghost var wit := SplitLeafOfIndexAtKey(node, childidx, pivot, nleft);
   //     pos := childidx as int64;
-  //     Spec.SplitChildOfIndexPreservesWF(old(I(node)), I(node), childidx as int, wit);
-  //     Spec.SplitChildOfIndexPreservesInterpretation(old(I(node)), I(node), childidx as int, wit);
-  //     Spec.SplitChildOfIndexPreservesAllKeys(old(I(node)), I(node), childidx as int, wit);
+  //     Model.SplitChildOfIndexPreservesWF(old(I(node)), I(node), childidx as int, wit);
+  //     Model.SplitChildOfIndexPreservesInterpretation(old(I(node)), I(node), childidx as int, wit);
+  //     Model.SplitChildOfIndexPreservesAllKeys(old(I(node)), I(node), childidx as int, wit);
   //   }
   // }
 
   // method EnsurePivotNotFull(node: Node, pivot: Key) returns (pos: int64)
   //   requires WFShape(node)
-  //   requires Spec.WF(I(node))
-  //   requires Spec.NumElements(I(node)) < Uint64UpperBound()
+  //   requires Model.WF(I(node))
+  //   requires Model.NumElements(I(node)) < Uint64UpperBound()
   //   requires node.contents.Index?
   //   requires !Full(node)
   //   ensures WFShape(node)
-  //   ensures Spec.WF(I(node))
+  //   ensures Model.WF(I(node))
   //   ensures -1 <= pos as int < node.contents.nchildren as int
   //   ensures 0 <= pos as int < node.contents.nchildren as int - 1 ==> node.contents.pivots[pos] == pivot
   // {
-  //   var childidx := Spec.Keys.ArrayLargestLtePlus1(node.contents.pivots, 0, node.contents.nchildren-1, pivot);
+  //   var childidx := Model.Keys.ArrayLargestLtePlus1(node.contents.pivots, 0, node.contents.nchildren-1, pivot);
   //   if 0 < childidx && node.contents.pivots[childidx-1] == pivot {
   //     pos := childidx as int64 - 1;
   //   } else {
@@ -884,12 +884,12 @@ abstract module MutableBtreeBulkOperations {
 
   // method EnsurePivot(node: Node, pivot: Key) returns (pos: int64)
   //   requires WFShape(node)
-  //   requires Spec.WF(I(node))
-  //   requires Spec.NumElements(I(node)) < Uint64UpperBound()
+  //   requires Model.WF(I(node))
+  //   requires Model.NumElements(I(node)) < Uint64UpperBound()
   //   requires node.contents.Index?
   //   requires !Full(node)
   //   ensures WFShape(node)
-  //   ensures Spec.WF(I(node))
+  //   ensures Model.WF(I(node))
   //   ensures -1 <= pos as int < node.contents.nchildren as int
   //   ensures 0 <= pos as int < node.contents.nchildren as int - 1 ==> node.contents.pivots[pos] == pivot
 
